IMP--_To_SAS+/SAS_Plus_Plus_Representation.thy
@@ -1,0 +1,130 @@
+(*
+  Author: Mohammad Abdulaziz, Fred Kurz, Florian Keßler
+*)
+theory SAS_Plus_Plus_Representation
+imports "Verified_SAT_Based_AI_Planning.SAS_Plus_Representation"
+begin
+
+section "SAS++ Representation"
+
+text \<open> We introduce SAS++, an adopted version of SAS+ that allows for partial initial states
+      where not all variables need to have a defined value. \<close>
+
+definition "is_valid_problem_sas_plus_plus \<Psi> 
+  \<equiv> let ops = operators_of \<Psi>
+      ; vs = variables_of \<Psi>
+      ; I = initial_of \<Psi>
+      ; G = goal_of \<Psi>
+      ; D = range_of \<Psi>
+    in list_all (\<lambda>v. D v \<noteq> None) vs
+    \<and> list_all (is_valid_operator_sas_plus \<Psi>) ops 
+    \<and> list_all (\<lambda> v. length (the (D v)) > 0) vs  
+    \<and> (\<forall>v. I v \<noteq> None \<longrightarrow> ListMem v vs) 
+    \<and> (\<forall>v. I v \<noteq> None \<longrightarrow> ListMem (the (I v)) (the (D v)))
+    \<and> (\<forall>v. G v \<noteq> None \<longrightarrow> ListMem v vs)
+    \<and> (\<forall>v. G v \<noteq> None \<longrightarrow> ListMem (the (G v)) (the (D v)))" 
+
+
+(* TODO can be replaced by proof for sublocale? *)
+lemma is_valid_problem_sas_plus_plus_then:
+  fixes \<Psi>::"('v,'d) sas_plus_problem"
+  assumes "is_valid_problem_sas_plus_plus \<Psi>"
+  shows "\<forall>v \<in> set ((\<Psi>)\<^sub>\<V>\<^sub>+). (\<R>\<^sub>+ \<Psi> v) \<noteq> {}"
+    and "\<forall>op \<in> set ((\<Psi>)\<^sub>\<O>\<^sub>+). is_valid_operator_sas_plus \<Psi> op"
+    and "dom ((\<Psi>)\<^sub>I\<^sub>+) \<subseteq> set ((\<Psi>)\<^sub>\<V>\<^sub>+)"
+    and "\<forall>v \<in> dom ((\<Psi>)\<^sub>I\<^sub>+). the (((\<Psi>)\<^sub>I\<^sub>+) v) \<in> \<R>\<^sub>+ \<Psi> v"
+    and "dom ((\<Psi>)\<^sub>G\<^sub>+) \<subseteq> set ((\<Psi>)\<^sub>\<V>\<^sub>+)"
+    and "\<forall>v \<in> dom ((\<Psi>)\<^sub>G\<^sub>+). the (((\<Psi>)\<^sub>G\<^sub>+) v) \<in> \<R>\<^sub>+ \<Psi> v" 
+proof -
+  let ?vs = "sas_plus_problem.variables_of \<Psi>"
+    and ?ops = "sas_plus_problem.operators_of \<Psi>"
+    and ?I = "sas_plus_problem.initial_of \<Psi>"
+    and ?G = "sas_plus_problem.goal_of \<Psi>"
+    and ?D = "sas_plus_problem.range_of \<Psi>"
+  {
+    fix v 
+    have "(?D v \<noteq> None \<and> ?D v \<noteq> Some []) \<longleftrightarrow> ((\<R>\<^sub>+ \<Psi> v) \<noteq> {})"
+      by (cases "?D v"; (auto simp: range_of'_def))
+  } note nb = this
+  have nb\<^sub>1: "\<forall>v \<in> set ?vs. ?D v \<noteq> None"
+    and nb\<^sub>4: "\<forall>v \<in> set ?vs. length (the (?D v)) > 0" 
+    and "\<forall>op \<in> set ?ops. is_valid_operator_sas_plus \<Psi> op"
+    and "\<forall>v. ?I v \<noteq> None \<longrightarrow> v \<in> set ?vs"
+    and nb\<^sub>2: "\<forall>v. ?I v \<noteq> None \<longrightarrow> the (?I v) \<in> set (the (?D v))"
+    and "\<forall>v. ?G v \<noteq> None \<longrightarrow> v \<in> set ?vs"
+    and nb\<^sub>3: "\<forall>v. ?G v \<noteq> None \<longrightarrow> the (?G v) \<in> set (the (?D v))"
+    using assms 
+    unfolding SAS_Plus_Plus_Representation.is_valid_problem_sas_plus_plus_def Let_def 
+      list_all_iff ListMem_iff 
+    by argo+
+  then have G3: "\<forall>op \<in> set ((\<Psi>)\<^sub>\<O>\<^sub>+). is_valid_operator_sas_plus \<Psi> op"
+    and G4: "dom ((\<Psi>)\<^sub>I\<^sub>+) \<subseteq> set ((\<Psi>)\<^sub>\<V>\<^sub>+)"
+    and G5: "dom ((\<Psi>)\<^sub>G\<^sub>+) \<subseteq> set ((\<Psi>)\<^sub>\<V>\<^sub>+)"
+    unfolding variables_of_def operators_of_def
+    by auto+
+  moreover {
+    fix v
+    assume "v \<in> set ((\<Psi>)\<^sub>\<V>\<^sub>+)"
+    then have "?D v \<noteq> None"
+      using nb\<^sub>1 
+      by force+
+  } note G6 = this
+  moreover {
+    fix v
+    assume "v \<in> set ((\<Psi>)\<^sub>\<V>\<^sub>+)"
+    then have "(\<R>\<^sub>+ \<Psi> v) \<noteq> {}"
+      using G6 nb\<^sub>4
+      by(auto simp: range_of'_def split: option.splits)
+  }
+  moreover {
+    fix v
+    assume "v \<in> dom ((\<Psi>)\<^sub>I\<^sub>+)"
+    moreover have "((\<Psi>)\<^sub>I\<^sub>+) v \<noteq> None"
+      using calculation
+      by blast+
+    moreover {
+      have "v \<in> set ((\<Psi>)\<^sub>\<V>\<^sub>+)"
+        using G4 calculation(1)
+        by fast
+      then have "sas_plus_problem.range_of \<Psi> v \<noteq> None" 
+        using range_of_not_empty
+        unfolding range_of'_def
+        using G6 
+        by fast+
+      hence "set (the (?D v)) = \<R>\<^sub>+ \<Psi> v" 
+        by (simp add: \<open>sas_plus_problem.range_of \<Psi> v \<noteq> None\<close> option.case_eq_if range_of'_def)
+    }
+    ultimately have "the (((\<Psi>)\<^sub>I\<^sub>+) v) \<in> \<R>\<^sub>+ \<Psi> v"
+      using nb\<^sub>2
+      by force
+  }
+  moreover {
+    fix v
+    assume "v \<in> dom ((\<Psi>)\<^sub>G\<^sub>+)"
+    then have "((\<Psi>)\<^sub>G\<^sub>+) v \<noteq> None"
+      by blast
+    moreover {
+      have "v \<in> set ((\<Psi>)\<^sub>\<V>\<^sub>+)"
+        using G5 calculation(1)
+        by fast
+      then have "sas_plus_problem.range_of \<Psi> v \<noteq> None" 
+        using range_of_not_empty
+        using G6
+        by fast+
+      hence "set (the (?D v)) = \<R>\<^sub>+ \<Psi> v" 
+        by (simp add: \<open>sas_plus_problem.range_of \<Psi> v \<noteq> None\<close> option.case_eq_if range_of'_def)
+    }
+    ultimately have "the (((\<Psi>)\<^sub>G\<^sub>+) v) \<in> \<R>\<^sub>+ \<Psi> v"
+      using nb\<^sub>3
+      by auto
+  }
+  ultimately show "\<forall>v \<in> set ((\<Psi>)\<^sub>\<V>\<^sub>+). (\<R>\<^sub>+ \<Psi> v) \<noteq> {}"
+    and "\<forall>op \<in> set((\<Psi>)\<^sub>\<O>\<^sub>+). is_valid_operator_sas_plus \<Psi> op"
+    and "dom ((\<Psi>)\<^sub>I\<^sub>+) \<subseteq> set ((\<Psi>)\<^sub>\<V>\<^sub>+)"
+    and "\<forall>v \<in> dom ((\<Psi>)\<^sub>I\<^sub>+). the (((\<Psi>)\<^sub>I\<^sub>+) v) \<in> \<R>\<^sub>+ \<Psi> v"
+    and "dom ((\<Psi>)\<^sub>G\<^sub>+) \<subseteq> set ((\<Psi>)\<^sub>\<V>\<^sub>+)"
+    and "\<forall>v \<in> dom ((\<Psi>)\<^sub>G\<^sub>+). the (((\<Psi>)\<^sub>G\<^sub>+) v) \<in> \<R>\<^sub>+ \<Psi> v"
+    by auto
+qed
+
+end
